\begin{enumerate}
    \item False
    \item By definition, 
    \begin{align}
        f_Y\brak{y} &=  \int_{-\infty}^{\infty} f(x,y) \,dx \\
        &= \int_{0}^{y} cxy \,dx \\
        &= cy \brak{\frac{x^2}{2}} \Biggr|_{0}^{y} \\
        &= \frac{ cy^3}{2}
    \end{align}
     \begin{align}
    \label{eq:: pdfy}
    \implies f_Y(y)  = 
    \begin{cases}
    \frac{ cy^3}{2}, &  0<y<1
    \\
    0 & \text{ otherwise. }
    \end{cases}
    \end{align}   
    $\because$ the area under the pdf is 1,  from \eqref{eq:: pdfy},
    \begin{align}
    \implies    \int_{-\infty}^{\infty} f_Y(y) \,dy &= 1 \\
    \implies        \int_{0}^{1} c\frac{y^3}{2} & =1 \\
    \implies    \frac{c}{8} &= 1 \\
    \text{or, }    c & = 8
    \end{align}
%
Also,
% The pdf of Y is 
 \begin{align}
\label{eq:: pdf_y}
f_Y(y)  = 
\begin{cases}
 4y^3 & \text{, if } 0<y<1
\\
0 & \text{, otherwise }
\end{cases}
\end{align}   

\item 
\begin{align}
    f_X\brak{x} &=  \int_{-\infty}^{\infty} f(x,y) \,dy \\
    &= \int_{x}^{1} cxy \,dy \\
    &= cx \brak{\frac{y^2}{2}} \Biggr|_{x}^{1} \\
    &= cx \brak{\frac{1- x^2}{2}}
\end{align}
%
\begin{align}
\label{eq:: pdf_x}
\implies f_X(x)  = 
\begin{cases}
4x \brak{1- x^2}, &  0<x<1
\\
0 & \text{ otherwise }
\end{cases}
\end{align} 
%
From \eqref{eq:: pdf_x} and \eqref{eq:: pdf_y}
\begin{align}
f_X(x) \times f_Y(y) & = 
\begin{cases}
16xy^3 \brak{1- x^2} & \text{, if } 0<x,y<1 
\\
0 & \text{, otherwise }
\end{cases}
\\
  &\neq f(x,y)
\end{align} 
%Since $f(x,y) $ and $ f_X(x) \times f_Y(y) $ are different, random variables 
Hence, $X$ and $Y$ are not independent. 
%Therefore option (3) is not correct. \\
\item
% The marginal PDF of X is given by,
% \begin{align}
% \label{eq:: pdf_x1}
% f_X(x)  = 
% \begin{cases}
% 4x \brak{1- x^2} & \text{, if } 0<x<1
% \\
% 0 & \text{, otherwise }
% \end{cases}
% \end{align} 
% The marginal CDF of X, $ F_X(x)$ is given by,
\begin{align}
    F_X(x) &=  \int_{-\infty}^{x} f_X(x) \,dx \\
    &= \int_{0}^{x} 4x(1-x^2) \,dx \\
     &= \int_{0}^{x} 4x-4x^3 \,dx \\
     & = 2x^2 - 4x^4 \text{ for }  0< x< 1
\end{align}
yielding
\begin{align}
\label{eq:: cdf_x}
F_X(x)  = 
\begin{cases}
0 &  x \le 0
\\
2x^2 - 4x^4    &  0 <x< 1
\\
1 &    x \ge 1
\end{cases}
\end{align}
From \eqref{eq:: cdf_x},
\begin{multline}
    \Pr\brak{Y- \epsilon < X < Y + \epsilon} 
    \\
    = F_X(Y + \epsilon) -  F_X(Y - \epsilon)  
    \\
     = 8\epsilon Y\brak{1 - Y^2 - \epsilon^2}
\end{multline}
upon simplification.  Letting
%
\begin{align}
g(Y)&= 8\epsilon Y(1 - Y^2 - \epsilon^2), \\
    E[g(Y)] &= \int_{-\infty}^{\infty} g(y) f_Y(y) \,dy 
    \\
     & = \int_{0}^{1} (4y^3) (8\epsilon y)(1 - y^2 - \epsilon^2) \,dy 
\end{align}
\begin{multline}
\implies     \Pr\brak{Y- \epsilon < X < Y + \epsilon}     \\
= 32\epsilon \brak{\frac{2- 7\epsilon^2}{35}}
\end{multline}
Now substituting $ \epsilon = 0 $ in the above, 
\begin{align}
    \pr{X =Y}  = 0
\end{align}
\end{enumerate}