From the given information, 
\begin{align}
    p_{X}(n) &= 
\begin{cases}
p & n=0
\\
1-p & n=1
\end{cases}\label{sum/1/1}
\\
p_{Y}(n) &= 
\begin{cases}
q & n=0
\\
1-q & n=1
\end{cases}\label{sum/1/2}
\end{align}
%
  The characteristic functions of $X$ and $Y$ are 
%
\begin{align}
\phi_X(z)&=\mean{z^{-X}} =  p+(1-p)z^{-1}
\\
\phi_Y(z)&= q+(1-q)z^{-1}
\end{align}
and the CF of $  Z=X+Y$ is 
\begin{align}
\phi_{X+Y}(z)&=\mean{z^{-(X+Y)}} \\
               &=\phi_X(z)\times \phi_Y(z)
               \\
  & =\sbrak{p+(1-p)z^{-1}}\sbrak{q+(1-q)z^{-1}}
  \end{align}
  \begin{multline}
\implies \phi_{Z}(z) = pq+(p+q-2pq)z^{-1}\\
  +(1-p)(1-q)z^{-2}
\end{multline}
yielding 
%   From equation \eqref{sum/1/1}, we get\\
%     The pmf of Z is 
\begin{align}
    p_{Z}(n) = 
\begin{cases}
pq & n=0
\\
p+q-2pq & n=1\\
(1-p)(1-q) & n=2
\end{cases}\label{sum/1/3}
\end{align}
Thus, 
\begin{align}
    \pr{X+Y\geq1} = 1 - \pr{Z<1}= 1-pq   
\end{align}